Use LowStar.Modifies instead of LowStar.Buffer in interop generation + Branch quad32_xor in Low.GCMencrypt

src/arch/x64/interop/Quad32_xor.fsti
@@ -21,6 +21,9 @@ open X64.Vale.Decls_i
 let b8 = B.buffer UInt8.t
 let s8 = B.buffer S8.t
 
+unfold let disjoint_or_eq (#a:Type0) (b1:B.buffer a) (b2:B.buffer a) =
+  M.(loc_disjoint (loc_buffer b1) (loc_buffer b2)) \/ b1 == b2 
+
 let rec loc_locs_disjoint_rec (l:s8) (ls:list s8) : Type0 =
   match ls with
   | [] -> True
@@ -47,7 +50,11 @@ let buffer_to_quad32 (b:s8 { B.length b % 16 == 0 /\ B.length b > 0 }) (h:HS.mem
   BV.sel h b128 0
 
 let pre_cond (h:HS.mem) (src1:s8) (src2:s8) (dst:s8) = 
-  live h src1 /\ live h src2 /\ live h dst /\ list_disjoint_or_eq [src1;src2;dst] /\  B.length src1 == 16 /\ B.length src2 == 16 /\ B.length dst == 16
+  live h src1 /\ live h src2 /\ live h dst /\ 
+  disjoint_or_eq src1 src2  /\
+  disjoint_or_eq src1 dst /\    
+  disjoint_or_eq src2 dst /\
+  B.length src1 == 16 /\ B.length src2 == 16 /\ B.length dst == 16
 
 let post_cond (h:HS.mem) (h':HS.mem) (src1:s8) (src2:s8) (dst:s8) = B.length src1 == 16 /\ B.length src2 == 16 /\ B.length dst == 16 /\
   M.modifies (M.loc_buffer dst) h h' /\
